SampCert/DifferentialPrivacy/Queries/UnboundedMax/Properties.lean
@@ -259,39 +259,36 @@ lemma sv1_sv2_eq ε₁ ε₂ l : sv1_privMax qs ε₁ ε₂ l = sv2_privMax qs �
   simp [sv1_privMax, sv2_privMax]
 
 
-/-
-
 
 /-
 ## Program version 3
   - Truncates the loop
 -/
 
-def sv3_loop (ε₁ ε₂ : ℕ+) (τ : ℤ) (l : List ℕ) (point : ℕ) (init : sv1_state) : SLang sv1_state := do
-  probWhileCut (sv1_privMaxC τ l) (sv1_privMaxF ε₁ ε₂) (point + 1) init
+def sv3_loop (qs : sv_query) (ε₁ ε₂ : ℕ+) (τ : ℤ) (l : List ℕ) (point : ℕ) (init : sv1_state) : SLang sv1_state := do
+  probWhileCut (sv1_privMaxC qs τ l) (sv1_privMaxF ε₁ ε₂) (point + 1) init
 
-def sv3_privMax (ε₁ ε₂ : ℕ+) (l : List ℕ) : SLang ℕ :=
+def sv3_privMax (qs : sv_query) (ε₁ ε₂ : ℕ+) (l : List ℕ) : SLang ℕ :=
   fun (point : ℕ) =>
   let computation : SLang ℕ := do
     let τ <- privNoiseThresh ε₁ ε₂
     let v0 <- privNoiseGuess ε₁ ε₂
-    let sk <- sv3_loop ε₁ ε₂ τ l point ([], v0)
+    let sk <- sv3_loop qs ε₁ ε₂ τ l point ([], v0)
     return (sv1_threshold sk)
   computation point
-
 
 def cone_of_possibility (cut : ℕ) (initial hist : List ℤ) : Prop :=
   (hist.length < cut + initial.length) ∧ (initial.length ≤ hist.length)
 
-def constancy_at {ε₁ ε₂ : ℕ+} {τ : ℤ} {data : List ℕ} {v0 vk : ℤ} (cut : ℕ) (initial hist : List ℤ) : Prop :=
-  probWhileCut (sv1_privMaxC τ data) (sv1_privMaxF ε₁ ε₂) (1 + cut) (initial, v0) (hist, vk) =
-  probWhileCut (sv1_privMaxC τ data) (sv1_privMaxF ε₁ ε₂) cut       (initial, v0) (hist, vk)
+def constancy_at {qs : sv_query} {ε₁ ε₂ : ℕ+} {τ : ℤ} {data : List ℕ} {v0 vk : ℤ} (cut : ℕ) (initial hist : List ℤ) : Prop :=
+  probWhileCut (sv1_privMaxC qs τ data) (sv1_privMaxF ε₁ ε₂) (1 + cut) (initial, v0) (hist, vk) =
+  probWhileCut (sv1_privMaxC qs τ data) (sv1_privMaxF ε₁ ε₂) cut       (initial, v0) (hist, vk)
 
 
 -- All points outside of the cone are zero
 lemma external_to_cone_zero :
     (¬ cone_of_possibility cut initial hist) ->
-    probWhileCut (sv1_privMaxC τ data) (sv1_privMaxF ε₁ ε₂) cut (initial, v0) (hist, vk) = 0 := by
+    probWhileCut (sv1_privMaxC qs τ data) (sv1_privMaxF ε₁ ε₂) cut (initial, v0) (hist, vk) = 0 := by
   revert initial v0 vk
   induction cut
   · simp [probWhileCut, probWhileFunctional]
@@ -325,10 +322,10 @@ lemma external_to_cone_zero :
       simp_all [cone_of_possibility]
 
 -- Base case: left edge of the cone satisfies constancy
-lemma cone_left_edge_constancy {ε₁ ε₂ : ℕ+} {τ : ℤ} {data : List ℕ} {v0 vk : ℤ} (cut : ℕ) (initial hist : List ℤ) :
+lemma cone_left_edge_constancy {qs} {ε₁ ε₂ : ℕ+} {τ : ℤ} {data : List ℕ} {v0 vk : ℤ} (cut : ℕ) (initial hist : List ℤ) :
     hist.length = initial.length ->
     cone_of_possibility cut initial hist ->
-    @constancy_at _ _ ε₁ ε₂ τ data v0 vk cut initial hist := by
+    @constancy_at _ _ qs ε₁ ε₂ τ data v0 vk cut initial hist := by
   intro Hlen Hcone
   -- cut > 0 due to cone
   cases cut
@@ -342,7 +339,7 @@ lemma cone_left_edge_constancy {ε₁ ε₂ : ℕ+} {τ : ℤ} {data : List ℕ}
   unfold probWhileCut
   unfold probWhileFunctional
 
-  cases (sv1_privMaxC τ data (initial, v0))
+  cases (sv1_privMaxC qs τ data (initial, v0))
   · -- False case: both programs terminate with initial state
     simp
   · -- True case: both programs step to a point outside of the cone, so are zero
@@ -378,10 +375,9 @@ lemma cone_left_edge_constancy {ε₁ ε₂ : ℕ+} {τ : ℤ} {data : List ℕ}
     rw [external_to_cone_zero (by simp_all [cone_of_possibility])]
     rw [external_to_cone_zero (by simp_all [cone_of_possibility])]
 
-
-lemma cone_constancy {ε₁ ε₂ : ℕ+} {τ : ℤ} {data : List ℕ} {v0 vk : ℤ} (cut : ℕ) (initial hist : List ℤ) :
+lemma cone_constancy {qs} {ε₁ ε₂ : ℕ+} {τ : ℤ} {data : List ℕ} {v0 vk : ℤ} (cut : ℕ) (initial hist : List ℤ) :
     cone_of_possibility cut initial hist ->
-    @constancy_at _ _ ε₁ ε₂ τ data v0 vk cut initial hist := by
+    @constancy_at _ _ qs ε₁ ε₂ τ data v0 vk cut initial hist := by
   -- Need theorem to be true for all initial states, since this will increase during the induction
   -- v0 and vk will also change in ways which don't matter
   revert initial v0 vk
@@ -392,7 +388,7 @@ lemma cone_constancy {ε₁ ε₂ : ℕ+} {τ : ℤ} {data : List ℕ} {v0 vk : 
     intro v0 vk initial Hcone
     unfold constancy_at
     simp [probWhileCut, probWhileFunctional]
-    cases (sv1_privMaxC τ data (initial, v0)) <;> simp
+    cases (sv1_privMaxC qs τ data (initial, v0)) <;> simp
     unfold cone_of_possibility at Hcone
     linarith
 
@@ -408,7 +404,7 @@ lemma cone_constancy {ε₁ ε₂ : ℕ+} {τ : ℤ} {data : List ℕ} {v0 vk : 
   unfold probWhileFunctional
 
   -- If the conditional is false, we are done
-  cases (sv1_privMaxC τ data (initial, v0))
+  cases (sv1_privMaxC qs τ data (initial, v0))
   · simp
 
 
@@ -464,7 +460,7 @@ lemma cone_constancy {ε₁ ε₂ : ℕ+} {τ : ℤ} {data : List ℕ} {v0 vk : 
     · trivial
 
 
-lemma sv2_sv3_eq ε₁ ε₂ l : sv2_privMax ε₁ ε₂ l = sv3_privMax ε₁ ε₂ l := by
+lemma sv2_sv3_eq (qs : sv_query) ε₁ ε₂ l : sv2_privMax qs ε₁ ε₂ l = sv3_privMax qs ε₁ ε₂ l := by
   apply SLang.ext
 
   -- Step through equal headers
@@ -514,7 +510,7 @@ lemma sv2_sv3_eq ε₁ ε₂ l : sv2_privMax ε₁ ε₂ l = sv3_privMax ε₁ �
         rename_i Hcont _
         apply Hcont
         linarith
-    have HK := @cone_constancy _ _ ε₁ ε₂ τ l v0 vk i [] hist
+    have HK := @cone_constancy _ _ qs ε₁ ε₂ τ l v0 vk i [] hist
     unfold constancy_at at HK
     conv =>
       enter [1, 3]
@@ -534,12 +530,12 @@ lemma sv2_sv3_eq ε₁ ε₂ l : sv2_privMax ε₁ ε₂ l = sv3_privMax ε₁ �
 
 
 -- Commute out a single sample from the loop
-lemma sv3_loop_unroll_1 (τ : ℤ) (ε₁ ε₂ : ℕ+) l point L vk :
-    sv3_loop ε₁ ε₂ τ l (point + 1) (L, vk) =
+lemma sv3_loop_unroll_1 qs (τ : ℤ) (ε₁ ε₂ : ℕ+) l point L vk :
+    sv3_loop qs ε₁ ε₂ τ l (point + 1) (L, vk) =
     (do
       let vk1 <- privNoiseGuess ε₁ ε₂
-      if (sv1_privMaxC τ l (L, vk))
-        then (sv3_loop ε₁ ε₂ τ l point (L ++ [vk], vk1))
+      if (sv1_privMaxC qs τ l (L, vk))
+        then (sv3_loop qs ε₁ ε₂ τ l point (L ++ [vk], vk1))
         else probPure (L, vk)) := by
   conv =>
     lhs
@@ -610,19 +606,19 @@ def sv4_privMaxF (s : sv4_state) : SLang sv4_state :=
   | [] => probZero
   | (p :: ps) => return ((s.1.1 ++ [s.1.2], p), ps)
 
-def sv4_privMaxC (τ : ℤ) (l : List ℕ) (st : sv4_state) : Bool := sv1_privMaxC τ l st.1
+def sv4_privMaxC (qs : sv_query) (τ : ℤ) (l : List ℕ) (st : sv4_state) : Bool := sv1_privMaxC qs τ l st.1
 
-def sv4_loop (ε₁ ε₂ : ℕ+) (τ : ℤ) (l : List ℕ) (point : ℕ) (init : sv1_state) : SLang sv1_state := do
+def sv4_loop (qs : sv_query) (ε₁ ε₂ : ℕ+) (τ : ℤ) (l : List ℕ) (point : ℕ) (init : sv1_state) : SLang sv1_state := do
   let presamples <- sv4_presample ε₁ ε₂ point
-  let v <- probWhileCut (sv4_privMaxC τ l) sv4_privMaxF (point + 1) (init, presamples)
+  let v <- probWhileCut (sv4_privMaxC qs τ l) sv4_privMaxF (point + 1) (init, presamples)
   return v.1
 
-lemma sv3_loop_unroll_1_alt (τ : ℤ) (ε₁ ε₂ : ℕ+) l point (initial_state : sv1_state) :
-    sv3_loop ε₁ ε₂ τ l (point + 1) initial_state =
+lemma sv3_loop_unroll_1_alt qs (τ : ℤ) (ε₁ ε₂ : ℕ+) l point (initial_state : sv1_state) :
+    sv3_loop qs ε₁ ε₂ τ l (point + 1) initial_state =
     (do
       let vk1 <- privNoiseGuess ε₁ ε₂
-      if (sv1_privMaxC τ l initial_state)
-        then (sv3_loop ε₁ ε₂ τ l point (initial_state.1 ++ [initial_state.2], vk1))
+      if (sv1_privMaxC qs τ l initial_state)
+        then (sv3_loop qs ε₁ ε₂ τ l point (initial_state.1 ++ [initial_state.2], vk1))
         else probPure initial_state) := by
   rcases initial_state with ⟨ _ , _ ⟩
   rw [sv3_loop_unroll_1]
@@ -736,7 +732,6 @@ lemma sv4_presample_eval' (ε₁ ε₂ : ℕ+) (n : ℕ) (s : { l : List ℤ // 
   trivial
 
 
-
 lemma vector_sum_merge n (f : ℤ × { l : List ℤ // l.length = n } -> ENNReal) :
     (∑'p, f p) = ∑'(p : {l : List ℤ // l.length = n + 1}), f (vsm_0 p, vsm_rest p) := by
   apply @tsum_eq_tsum_of_ne_zero_bij
@@ -757,7 +752,6 @@ lemma vector_sum_merge n (f : ℤ × { l : List ℤ // l.length = n } -> ENNReal
     simp
     exists HL
   · simp [Function.support, DFunLike.coe]
-
 
 
 -- Split in the other order, used as a helper function
@@ -1090,8 +1084,8 @@ lemma presample_norm_lemma  (point : ℕ) (ε₁ ε₂ : ℕ+) :
     apply HasSum.tsum_eq S
 
 
-def sv3_sv4_loop_eq (ε₁ ε₂ : ℕ+) (τ : ℤ) (l : List ℕ) (point : ℕ) (init : sv1_state) :
-    sv3_loop ε₁ ε₂ τ l point init = sv4_loop ε₁ ε₂ τ l point init := by
+def sv3_sv4_loop_eq qs (ε₁ ε₂ : ℕ+) (τ : ℤ) (l : List ℕ) (point : ℕ) (init : sv1_state) :
+    sv3_loop qs ε₁ ε₂ τ l point init = sv4_loop qs ε₁ ε₂ τ l point init := by
   revert init
   induction point
   · -- It's a mess but it works
@@ -1143,13 +1137,13 @@ def sv3_sv4_loop_eq (ε₁ ε₂ : ℕ+) (τ : ℤ) (l : List ℕ) (point : ℕ)
     let ApplyIH :
       ((do
         let vk1 ← privNoiseGuess ε₁ ε₂
-        if sv1_privMaxC τ l init = true
-          then sv3_loop ε₁ ε₂ τ l point (init.1 ++ [init.2], vk1)
+        if sv1_privMaxC qs τ l init = true
+          then sv3_loop qs ε₁ ε₂ τ l point (init.1 ++ [init.2], vk1)
           else (SLang.probPure init) : SLang _) =
       ((do
         let vk1 ← privNoiseGuess ε₁ ε₂
-        if sv1_privMaxC τ l init = true
-          then sv4_loop ε₁ ε₂ τ l point (init.1 ++ [init.2], vk1)
+        if sv1_privMaxC qs τ l init = true
+          then sv4_loop qs ε₁ ε₂ τ l point (init.1 ++ [init.2], vk1)
           else probPure init) : SLang _)) := by
       simp
       apply SLang.ext
@@ -1164,15 +1158,14 @@ def sv3_sv4_loop_eq (ε₁ ε₂ : ℕ+) (τ : ℤ) (l : List ℕ) (point : ℕ)
 
     rw [ApplyIH]
     clear ApplyIH IH
-
     have ToPresample :
         (do
           let vk1 ← privNoiseGuess ε₁  ε₂
-          if sv1_privMaxC τ l init = true then sv4_loop ε₁ ε₂ τ l point (init.1 ++ [init.2], vk1) else probPure init) =
+          if sv1_privMaxC qs τ l init = true then sv4_loop qs ε₁ ε₂ τ l point (init.1 ++ [init.2], vk1) else probPure init) =
         (do
           let vps ← sv4_presample ε₁ ε₂ 1
           let vk1 := len_1_list_to_val vps
-          if sv1_privMaxC τ l init = true then sv4_loop ε₁ ε₂ τ l point (init.1 ++ [init.2], vk1) else probPure init) := by
+          if sv1_privMaxC qs τ l init = true then sv4_loop qs ε₁ ε₂ τ l point (init.1 ++ [init.2], vk1) else probPure init) := by
       apply SLang.ext
       intro final_state
       simp
@@ -1285,18 +1278,17 @@ def sv3_sv4_loop_eq (ε₁ ε₂ : ℕ+) (τ : ℤ) (l : List ℕ) (point : ℕ)
         apply presample_norm_lemma
       · simp
 
-
-def sv4_privMax (ε₁ ε₂ : ℕ+) (l : List ℕ) : SLang ℕ :=
+def sv4_privMax (qs : sv_query) (ε₁ ε₂ : ℕ+) (l : List ℕ) : SLang ℕ :=
   fun (point : ℕ) =>
   let computation : SLang ℕ := do
     let τ <- privNoiseThresh ε₁ ε₂
     let v0 <- privNoiseGuess ε₁ ε₂
-    let sk <- sv4_loop ε₁ ε₂ τ l point ([], v0)
+    let sk <- sv4_loop qs ε₁ ε₂ τ l point ([], v0)
     return (sv1_threshold sk)
   computation point
 
-def sv3_sv4_eq (ε₁ ε₂ : ℕ+) (l : List ℕ) :
-    sv3_privMax ε₁ ε₂ l = sv4_privMax ε₁ ε₂ l := by
+def sv3_sv4_eq qs (ε₁ ε₂ : ℕ+) (l : List ℕ) :
+    sv3_privMax qs ε₁ ε₂ l = sv4_privMax qs ε₁ ε₂ l := by
     unfold sv3_privMax
     unfold sv4_privMax
     simp
@@ -1304,34 +1296,32 @@ def sv3_sv4_eq (ε₁ ε₂ : ℕ+) (l : List ℕ) :
       enter [1, x, 1, y, 2, 1, z]
       rw [sv3_sv4_loop_eq]
 
-
 /-
 ## Program version 5
   - Executable
   - Isolates the loop for the next step
 -/
 
-def sv5_loop (τ : ℤ) (l : List ℕ) (point : ℕ) (init : sv4_state) : SLang ℕ := do
-  let sk <- probWhileCut (sv4_privMaxC τ l) sv4_privMaxF (point + 1) init
+def sv5_loop (qs : sv_query) (τ : ℤ) (l : List ℕ) (point : ℕ) (init : sv4_state) : SLang ℕ := do
+  let sk <- probWhileCut (sv4_privMaxC qs τ l) sv4_privMaxF (point + 1) init
   return (sv1_threshold sk.1)
 
-def sv5_privMax (ε₁ ε₂ : ℕ+) (l : List ℕ) : SLang ℕ :=
+def sv5_privMax (qs : sv_query) (ε₁ ε₂ : ℕ+) (l : List ℕ) : SLang ℕ :=
   fun (point : ℕ) =>
   let computation : SLang ℕ := do
     let τ <- privNoiseThresh ε₁ ε₂
     let v0 <- privNoiseGuess ε₁ ε₂
     let presamples <- sv4_presample ε₁ ε₂ point
-    @sv5_loop τ l point (([], v0), presamples)
+    @sv5_loop qs τ l point (([], v0), presamples)
   computation point
 
-def sv4_sv5_eq (ε₁ ε₂ : ℕ+) (l : List ℕ) :
-    sv4_privMax ε₁ ε₂ l = sv5_privMax ε₁ ε₂ l := by
+def sv4_sv5_eq (qs : sv_query) (ε₁ ε₂ : ℕ+) (l : List ℕ) :
+    sv4_privMax qs ε₁ ε₂ l = sv5_privMax qs ε₁ ε₂ l := by
   unfold sv4_privMax
   unfold sv5_privMax
   unfold sv4_loop
   unfold sv5_loop
   simp
-
 
 
 /-
@@ -1359,17 +1349,17 @@ def is_past_configuration (sp sc : sv4_state) : Prop :=
   (sp.1.1.length ≤ sc.1.1.length) ∧ sp.1.1 ++ [sp.1.2] ++ sp.2 = sc.1.1 ++ [sc.1.2] ++ sc.2
 
 -- All past configurations had their loop check execute to True
-def sv6_privMax_hist (τ : ℤ) (l : List ℕ) (s : sv4_state) : Prop :=
-  ∀ sp, (is_past_configuration sp s) -> sv4_privMaxC τ l sp = true
+def sv6_privMax_hist (qs : sv_query) (τ : ℤ) (l : List ℕ) (s : sv4_state) : Prop :=
+  ∀ sp, (is_past_configuration sp s) -> sv4_privMaxC qs τ l sp = true
 
 
 -- If all past configurations of sp evaluate to True,
 -- and the next one evaluates to true,
 -- then all past configurations for the next one evaluate to True
-lemma sv6_privMax_hist_step (τ : ℤ) (l : List ℕ) (past fut_rest : List ℤ) (present fut : ℤ) :
-    sv6_privMax_hist τ l ((past, present), fut :: fut_rest) ->
-    sv4_privMaxC τ l ((past ++ [present], fut), fut_rest) ->
-    sv6_privMax_hist τ l ((past ++ [present], fut), fut_rest) := by
+lemma sv6_privMax_hist_step (qs : sv_query) (τ : ℤ) (l : List ℕ) (past fut_rest : List ℤ) (present fut : ℤ) :
+    sv6_privMax_hist qs τ l ((past, present), fut :: fut_rest) ->
+    sv4_privMaxC qs τ l ((past ++ [present], fut), fut_rest) ->
+    sv6_privMax_hist qs τ l ((past ++ [present], fut), fut_rest) := by
   intro H1 H2
   unfold sv6_privMax_hist
   intro s H3
@@ -1404,13 +1394,13 @@ def is_past_configuration_strict (sp sc : sv4_state) : Prop :=
   (sp.1.1.length < sc.1.1.length) ∧ sp.1.1 ++ [sp.1.2] ++ sp.2 = sc.1.1 ++ [sc.1.2] ++ sc.2
 
 -- All strictly past configurations had their loop check execute to True
-def sv6_privMax_hist_strict (τ : ℤ) (l : List ℕ) (s : sv4_state) : Prop :=
-  ∀ sp, (is_past_configuration_strict sp s) -> sv4_privMaxC τ l sp = true
+def sv6_privMax_hist_strict (qs : sv_query) (τ : ℤ) (l : List ℕ) (s : sv4_state) : Prop :=
+  ∀ sp, (is_past_configuration_strict sp s) -> sv4_privMaxC qs τ l sp = true
 
-lemma sv6_privMax_hist_step_strict (τ : ℤ) (l : List ℕ) (past fut_rest : List ℤ) (present fut : ℤ) :
-    sv6_privMax_hist_strict τ l ((past, present), fut :: fut_rest) ->
-    sv4_privMaxC τ l ((past, present), fut :: fut_rest) ->
-    sv6_privMax_hist_strict τ l ((past ++ [present], fut), fut_rest) := by
+lemma sv6_privMax_hist_step_strict (qs : sv_query) (τ : ℤ) (l : List ℕ) (past fut_rest : List ℤ) (present fut : ℤ) :
+    sv6_privMax_hist_strict qs τ l ((past, present), fut :: fut_rest) ->
+    sv4_privMaxC qs τ l ((past, present), fut :: fut_rest) ->
+    sv6_privMax_hist_strict qs τ l ((past ++ [present], fut), fut_rest) := by
   intro H1 H2
   unfold sv6_privMax_hist_strict
   intro s H3
@@ -1439,28 +1429,27 @@ lemma sv6_privMax_hist_step_strict (τ : ℤ) (l : List ℕ) (past fut_rest : Li
     rename_i s11 s12
     simp_all
 
-
 @[simp]
-def sv6_cond_rec (τ : ℤ) (l : List ℕ) (past : List ℤ) (pres : ℤ) (future : List ℤ) : Bool :=
+def sv6_cond_rec (qs : sv_query) (τ : ℤ) (l : List ℕ) (past : List ℤ) (pres : ℤ) (future : List ℤ) : Bool :=
   match future with
-  | [] => ¬ (sv4_privMaxC τ l ((past, pres), []))
-  | (f :: ff) => (sv4_privMaxC τ l ((past, pres), f :: ff) = true) && (sv6_cond_rec τ l (past ++ [pres]) f ff)
+  | [] => ¬ (sv4_privMaxC qs τ l ((past, pres), []))
+  | (f :: ff) => (sv4_privMaxC qs τ l ((past, pres), f :: ff) = true) && (sv6_cond_rec qs τ l (past ++ [pres]) f ff)
 
 @[simp]
-def sv6_cond (τ : ℤ) (l : List ℕ) (init : sv4_state) : Bool :=
-  sv6_cond_rec τ l init.1.1 init.1.2 init.2
+def sv6_cond (qs : sv_query) (τ : ℤ) (l : List ℕ) (init : sv4_state) : Bool :=
+  sv6_cond_rec qs τ l init.1.1 init.1.2 init.2
 
-def sv6_loop (τ : ℤ) (l : List ℕ) (point : ℕ) (init : sv4_state) : SLang ℕ := do
-  if (sv6_cond τ l init)
+def sv6_loop (qs : sv_query) (τ : ℤ) (l : List ℕ) (point : ℕ) (init : sv4_state) : SLang ℕ := do
+  if (sv6_cond qs τ l init)
     then return point
     else probZero
 
 -- QUESTION: What do we need for equality in the base case?
-lemma sv5_sv6_loop_base_case  (τ : ℤ) (l : List ℕ) (point eval : ℕ) (past future : List ℤ) (pres : ℤ) :
+lemma sv5_sv6_loop_base_case (qs : sv_query) (τ : ℤ) (l : List ℕ) (point eval : ℕ) (past future : List ℤ) (pres : ℤ) :
     future = [] ->
     List.length future = eval ->
     List.length (past ++ [pres] ++ future) = point + 1 ->
-    (sv6_loop τ l point ((past, pres), future)) point = (sv5_loop τ l eval ((past, pres), future)) point := by
+    (sv6_loop qs τ l point ((past, pres), future)) point = (sv5_loop qs τ l eval ((past, pres), future)) point := by
   intro Hfuture Heval Hstate
   rw [Hfuture]
   simp_all
@@ -1491,13 +1480,13 @@ lemma sv5_sv6_loop_base_case  (τ : ℤ) (l : List ℕ) (point eval : ℕ) (past
     aesop
 
 -- QUESTION: What do we need for sv6_loop to be equal to sv6_loop_cond (next)
-lemma sv6_loop_ind (τ : ℤ) (l : List ℕ) (point : ℕ) (past ff: List ℤ) (pres f: ℤ) :
-      (sv4_privMaxC τ l ((past, pres), f :: ff) = true) ->
+lemma sv6_loop_ind (qs : sv_query) (τ : ℤ) (l : List ℕ) (point : ℕ) (past ff: List ℤ) (pres f: ℤ) :
+      (sv4_privMaxC qs τ l ((past, pres), f :: ff) = true) ->
       List.length (past ++ [pres] ++ f :: ff) = point + 1 ->
-      (sv6_loop τ l point ((past, pres), f :: ff)) point = (sv6_loop τ l point ((past ++ [pres], f), ff)) point := by
+      (sv6_loop qs τ l point ((past, pres), f :: ff)) point = (sv6_loop qs τ l point ((past ++ [pres], f), ff)) point := by
   intro Hcondition _
   unfold sv6_loop
-  suffices (sv6_cond τ l ((past, pres), f :: ff) = sv6_cond τ l ((past ++ [pres], f), ff)) by
+  suffices (sv6_cond qs τ l ((past, pres), f :: ff) = sv6_cond qs τ l ((past ++ [pres], f), ff)) by
     split <;> split <;> try rfl
     all_goals simp_all
   conv =>
@@ -1508,9 +1497,9 @@ lemma sv6_loop_ind (τ : ℤ) (l : List ℕ) (point : ℕ) (past ff: List ℤ) (
 
 
 -- QUESTION: What do we need for sv5 to be equal to sv5_loop_cond (next) evaluated at point
-lemma sv5_loop_ind (τ : ℤ) (l : List ℕ) (eval point : ℕ) (past ff: List ℤ) (pres f: ℤ) :
-      (sv4_privMaxC τ l ((past, pres), f :: ff) = true) ->
-      (sv5_loop τ l (eval + 1) ((past, pres), f :: ff)) point = (sv5_loop τ l eval ((past ++ [pres], f), ff)) point := by
+lemma sv5_loop_ind (qs : sv_query) (τ : ℤ) (l : List ℕ) (eval point : ℕ) (past ff: List ℤ) (pres f: ℤ) :
+      (sv4_privMaxC qs τ l ((past, pres), f :: ff) = true) ->
+      (sv5_loop qs τ l (eval + 1) ((past, pres), f :: ff)) point = (sv5_loop qs τ l eval ((past ++ [pres], f), ff)) point := by
   intro Hcondition
   conv =>
     lhs
@@ -1524,30 +1513,28 @@ lemma sv5_loop_ind (τ : ℤ) (l : List ℕ) (eval point : ℕ) (past ff: List �
   · exfalso
     trivial
 
-
-def sv6_privMax (ε₁ ε₂ : ℕ+) (l : List ℕ) : SLang ℕ :=
+def sv6_privMax (qs : sv_query) (ε₁ ε₂ : ℕ+) (l : List ℕ) : SLang ℕ :=
   fun (point : ℕ) =>
   let computation : SLang ℕ := do
     let τ <- privNoiseThresh ε₁ ε₂
     let v0 <- privNoiseGuess ε₁ ε₂
     let presamples <- sv4_presample ε₁ ε₂ point
-    @sv6_loop τ l point (([], v0), presamples)
+    @sv6_loop qs τ l point (([], v0), presamples)
   computation point
 
 
-
 -- sv6_loop and sv5_loop are equal at point (under some conditions)
-def sv5_sv6_loop_eq_point (τ : ℤ) (l : List ℕ) (point eval : ℕ) (past future : List ℤ) (pres : ℤ) :
+def sv5_sv6_loop_eq_point (qs : sv_query) (τ : ℤ) (l : List ℕ) (point eval : ℕ) (past future : List ℤ) (pres : ℤ) :
     List.length (past ++ [pres] ++ future) = point + 1 ->
     List.length future = eval ->
     -- sv6_privMax_hist_strict τ l ((past, pres), future) ->
-    @sv5_loop τ l eval ((past, pres), future) point = @sv6_loop τ l point ((past, pres), future) point := by
+    @sv5_loop qs τ l eval ((past, pres), future) point = @sv6_loop qs τ l point ((past, pres), future) point := by
   revert past pres eval
   induction future
   · intro eval past pres H1 H2
     symm
     simp at H1
-    apply (sv5_sv6_loop_base_case _ _ _ _ _ _ _ (by rfl) H2 ?G2)
+    apply (sv5_sv6_loop_base_case _ _ _ _ _ _ _ _ (by rfl) H2 ?G2)
     case G2 =>
       simp
       trivial
@@ -1557,10 +1544,10 @@ def sv5_sv6_loop_eq_point (τ : ℤ) (l : List ℕ) (point eval : ℕ) (past fut
     · simp at Heval
 
     rename_i eval
-    cases (Classical.em (sv4_privMaxC τ l ((past, pres), f :: ff) = true))
+    cases (Classical.em (sv4_privMaxC qs τ l ((past, pres), f :: ff) = true))
     · rename_i Hcondition
-      rw [sv5_loop_ind _ _ _ _ _ _ _ _ Hcondition]
-      rw [sv6_loop_ind _ _ _ _ _ _ _ Hcondition Hstate]
+      rw [sv5_loop_ind _ _ _ _ _ _ _ _ _ Hcondition]
+      rw [sv6_loop_ind _ _ _ _ _ _ _ _ Hcondition Hstate]
       apply (IH eval (past ++ [pres]) f ?G1 ?G2)
       case G1 => simp_all
       case G2 => simp_all
@@ -1577,8 +1564,8 @@ def sv5_sv6_loop_eq_point (τ : ℤ) (l : List ℕ) (point eval : ℕ) (past fut
     simp_all [sv1_threshold]
 
 
-def sv5_sv6_eq (ε₁ ε₂ : ℕ+) (l : List ℕ) :
-    sv5_privMax ε₁ ε₂ l = sv6_privMax ε₁ ε₂ l := by
+def sv5_sv6_eq (qs : sv_query) (ε₁ ε₂ : ℕ+) (l : List ℕ) :
+    sv5_privMax qs ε₁ ε₂ l = sv6_privMax qs ε₁ ε₂ l := by
   unfold sv5_privMax
   unfold sv6_privMax
   apply SLang.ext
@@ -1604,27 +1591,26 @@ Not executable
 Separates out the zero case
 -/
 
-def sv7_privMax (ε₁ ε₂ : ℕ+) (l : List ℕ) : SLang ℕ :=
+def sv7_privMax (qs : sv_query) (ε₁ ε₂ : ℕ+) (l : List ℕ) : SLang ℕ :=
   fun (point : ℕ) =>
   let computation : SLang ℕ := do
     let τ <- privNoiseThresh ε₁ ε₂
     let v0 <- privNoiseGuess ε₁ ε₂
     match point with
     | 0 =>
-      if (¬ (sv4_privMaxC τ l (([], v0), [])))
+      if (¬ (sv4_privMaxC qs τ l (([], v0), [])))
         then probPure point
         else probZero
     | (Nat.succ point') => do
       let presamples <- sv4_presample ε₁ ε₂ point'
       let vk <- privNoiseGuess ε₁ ε₂
-      if (sv6_cond τ l (([], v0), presamples ++ [vk]))
+      if (sv6_cond qs τ l (([], v0), presamples ++ [vk]))
         then probPure point
         else probZero
   computation point
 
-
-def sv6_sv7_eq (ε₁ ε₂ : ℕ+) (l : List ℕ) :
-    sv6_privMax ε₁ ε₂ l = sv7_privMax ε₁ ε₂ l := by
+def sv6_sv7_eq (qs : sv_query) (ε₁ ε₂ : ℕ+) (l : List ℕ) :
+    sv6_privMax qs ε₁ ε₂ l = sv7_privMax qs ε₁ ε₂ l := by
   apply SLang.ext
   intro point
   unfold sv6_privMax
@@ -1735,39 +1721,40 @@ Defines G from the paper
 
 
 
-def sv8_sum (l : List ℕ) (past : List ℤ) (pres : ℤ) : ℤ := exactDiffSum (List.length past) l + pres
+def sv8_sum (qs : sv_query) (l : List ℕ) (past : List ℤ) (pres : ℤ) : ℤ :=
+  qs (List.length past) l + pres
+  -- exactDiffSum (List.length past) l + pres
 
 -- G is the maximum value of sv8_sum over the tape
-def sv8_G  (l : List ℕ) (past : List ℤ) (pres : ℤ) (future : List ℤ) : ℤ :=
+def sv8_G (qs : sv_query) (l : List ℕ) (past : List ℤ) (pres : ℤ) (future : List ℤ) : ℤ :=
   match future with
-  | []        => sv8_sum l past pres
-  | (f :: ff) => max (sv8_sum l past pres) (sv8_G l (past ++ [pres]) f ff)
+  | []        => sv8_sum qs l past pres
+  | (f :: ff) => max (sv8_sum qs l past pres) (sv8_G qs l (past ++ [pres]) f ff)
 
- def sv8_cond (τ : ℤ) (l : List ℕ) (past : List ℤ) (pres : ℤ) (future : List ℤ) (last : ℤ) : Bool :=
-   (sv8_G l past pres future < τ) ∧ (sv8_sum l (past ++ [pres] ++ future) last ≥ τ)
+ def sv8_cond (qs : sv_query) (τ : ℤ) (l : List ℕ) (past : List ℤ) (pres : ℤ) (future : List ℤ) (last : ℤ) : Bool :=
+   (sv8_G qs l past pres future < τ) ∧ (sv8_sum qs l (past ++ [pres] ++ future) last ≥ τ)
 
-def sv8_privMax (ε₁ ε₂ : ℕ+) (l : List ℕ) : SLang ℕ :=
+def sv8_privMax (qs : sv_query) (ε₁ ε₂ : ℕ+) (l : List ℕ) : SLang ℕ :=
   fun (point : ℕ) =>
   let computation : SLang ℕ := do
     let τ <- privNoiseThresh ε₁ ε₂
     let v0 <- privNoiseGuess ε₁ ε₂
     match point with
     | 0 =>
-      if (sv8_sum l [] v0 ≥ τ)
+      if (sv8_sum qs l [] v0 ≥ τ)
         then probPure point
         else probZero
     | (Nat.succ point') => do
       let presamples <- sv4_presample ε₁ ε₂ point'
       let vk <- privNoiseGuess ε₁ ε₂
-      if (sv8_cond τ l [] v0 presamples vk)
+      if (sv8_cond qs τ l [] v0 presamples vk)
         then probPure point
         else probZero
   computation point
 
-
-lemma sv7_sv8_cond_eq (τ : ℤ) (l : List ℕ) (v0 : ℤ) (vs : List ℤ) (vk : ℤ) :
-    sv8_cond τ l [] v0 vs vk = sv6_cond τ l (([], v0), vs ++ [vk]) := by
-  suffices (∀ init, sv8_cond τ l init v0 vs vk = sv6_cond τ l ((init, v0), vs ++ [vk])) by
+lemma sv7_sv8_cond_eq (qs : sv_query) (τ : ℤ) (l : List ℕ) (v0 : ℤ) (vs : List ℤ) (vk : ℤ) :
+    sv8_cond qs τ l [] v0 vs vk = sv6_cond qs τ l (([], v0), vs ++ [vk]) := by
+  suffices (∀ init, sv8_cond qs τ l init v0 vs vk = sv6_cond qs τ l ((init, v0), vs ++ [vk])) by
     apply this
   revert v0
   unfold sv8_cond
@@ -1786,16 +1773,16 @@ lemma sv7_sv8_cond_eq (τ : ℤ) (l : List ℕ) (v0 : ℤ) (vs : List ℤ) (vk :
       simp [sv6_cond_rec]
     rw [<- IH']
     clear IH'
-    cases (decide (τ ≤ sv8_sum l (init ++ vi :: vi_1 :: rest) vk)) <;> simp
+    cases (decide (τ ≤ sv8_sum qs l (init ++ vi :: vi_1 :: rest) vk)) <;> simp
     conv =>
       lhs
       unfold sv8_G
       simp
-    cases (decide (sv8_G l (init ++ [vi]) vi_1 rest < τ)) <;> simp
+    cases (decide (sv8_G qs l (init ++ [vi]) vi_1 rest < τ)) <;> simp
     simp [sv4_privMaxC, sv1_privMaxC, sv8_sum, sv1_threshold, sv1_noise]
 
-def sv7_sv8_eq (ε₁ ε₂ : ℕ+) (l : List ℕ) :
-    sv7_privMax ε₁ ε₂ l = sv8_privMax ε₁ ε₂ l := by
+def sv7_sv8_eq (qs : sv_query) (ε₁ ε₂ : ℕ+) (l : List ℕ) :
+    sv7_privMax qs ε₁ ε₂ l = sv8_privMax qs ε₁ ε₂ l := by
   apply SLang.ext
   intro point
   unfold sv7_privMax
@@ -1808,7 +1795,6 @@ def sv7_sv8_eq (ε₁ ε₂ : ℕ+) (l : List ℕ) :
   simp only [sv7_sv8_cond_eq, sv6_cond]
 
 
-
 /-
 ## Program v9
 
@@ -1817,14 +1803,14 @@ Rewritten so that the randomness we will cancel out is right at the front
 -/
 
 
-def sv9_privMax (ε₁ ε₂ : ℕ+) (l : List ℕ) : SLang ℕ :=
+def sv9_privMax (qs : sv_query) (ε₁ ε₂ : ℕ+) (l : List ℕ) : SLang ℕ :=
   fun (point : ℕ) =>
   let computation : SLang ℕ := do
     match point with
     | 0 => do
       let τ <- privNoiseThresh ε₁ ε₂
       let v0 <- privNoiseGuess ε₁ ε₂
-      if (sv8_sum l [] v0 ≥ τ)
+      if (sv8_sum qs l [] v0 ≥ τ)
         then probPure point
         else probZero
     | (Nat.succ point') => do
@@ -1832,13 +1818,13 @@ def sv9_privMax (ε₁ ε₂ : ℕ+) (l : List ℕ) : SLang ℕ :=
       let presamples <- sv4_presample ε₁ ε₂ point'
       let τ <- privNoiseThresh ε₁ ε₂
       let vk <- privNoiseGuess ε₁ ε₂
-      if (sv8_cond τ l [] v0 presamples vk)
+      if (sv8_cond qs τ l [] v0 presamples vk)
         then probPure point
         else probZero
   computation point
 
-def sv8_sv9_eq (ε₁ ε₂ : ℕ+) (l : List ℕ) :
-    sv8_privMax ε₁ ε₂ l = sv9_privMax ε₁ ε₂ l := by
+def sv8_sv9_eq (qs : sv_query) (ε₁ ε₂ : ℕ+) (l : List ℕ) :
+    sv8_privMax qs ε₁ ε₂ l = sv9_privMax qs ε₁ ε₂ l := by
   apply SLang.ext
   intro point
   unfold sv8_privMax
@@ -1995,7 +1981,8 @@ lemma exactDiffSum_append : exactDiffSum i (A ++ B) = exactDiffSum i A + exactDi
   rw [exactClippedSum_append]
   linarith
 
-lemma sv8_sum_append : sv8_sum (A ++ B) vp v0 = sv8_sum A vp v0 + sv8_sum B vp v0 - v0 := by
+/-
+lemma sv8_sum_append qs : sv8_sum (A ++ B) vp v0 = sv8_sum A vp v0 + sv8_sum B vp v0 - v0 := by
   simp [sv8_sum]
   simp [exactDiffSum_append]
   linarith
